src/Analysis/Solver/TD_Side_IP_Interface.thy
@@ -8,7 +8,7 @@ text \<open>
   Side-effecting TD backend for the interprocedural CFG (TD_side on
   side_cfg_T_ip).  Packages side_cfg_T_ip as cfg_side_T_ip_pkg, interprets it
   as TD_side_mono, reads back the stable set and unknown assignment
-  (side_stabl_at / side_sigma_at), and exposes the combined env (side_env_at).
+  (side_stabl_at / side_nu_at), and exposes the combined env (side_env_at).
 
   Monotonicity of side_cfg_T_ip is derived from transfer-function monotonicity
   (side_cfg_T_ip_is_mono_eq / _mono_sides / _mono_deps in TD_Side_IP_Mono).
@@ -50,39 +50,39 @@ qed
 definition side_stabl_at :: "pp \<Rightarrow> pp set"
   where "side_stabl_at x = fst (side.solve x)"
 
-definition side_sigma_at :: "pp \<Rightarrow> pp + unit \<Rightarrow> 'a abs_state"
-  where "side_sigma_at x = snd (side.solve x)"
+definition side_nu_at :: "pp \<Rightarrow> pp + unit \<Rightarrow> 'a abs_state"
+  where "side_nu_at x = snd (side.solve x)"
 
 definition side_env_at :: "pp \<Rightarrow> pp \<Rightarrow> 'a abs_state"
-  where "side_env_at x0 v = side_env (side_sigma_at x0) v"
+  where "side_env_at x0 v = side_env (side_nu_at x0) v"
 
 (* Combined env at the CFG entry, queried from the entry node. *)
 definition side_env_entry :: "pp \<Rightarrow> 'a abs_state"
   where "side_env_entry v = side_env_at (cfg_entry g) v"
 
-lemma side_sigma_at_solve:
-  "side_sigma_at x = snd (side.solve x)"
-  unfolding side_sigma_at_def by simp
+lemma side_nu_at_solve:
+  "side_nu_at x = snd (side.solve x)"
+  unfolding side_nu_at_def by simp
 
 lemma side_stabl_at_solve:
   "side_stabl_at x = fst (side.solve x)"
   unfolding side_stabl_at_def by simp
 
 lemma side_solve_prod:
-  "side.solve x = (side_stabl_at x, side_sigma_at x)"
-  unfolding side_stabl_at_def side_sigma_at_def
+  "side.solve x = (side_stabl_at x, side_nu_at x)"
+  unfolding side_stabl_at_def side_nu_at_def
   by (rule prod_eqI) simp_all
 
 lemma side_part_post_solution_at:
   assumes dom: "side.solve_dom x"
-  shows "part_post_solution cfg_side_T_ip_pkg x (side_sigma_at x) (side_stabl_at x)"
+  shows "part_post_solution cfg_side_T_ip_pkg x (side_nu_at x) (side_stabl_at x)"
 proof -
   from side.least_partial_post_solution[OF dom side_solve_prod] show ?thesis by simp
 qed
 
 lemma side_part_solution_at:
   assumes dom: "side.solve_dom x"
-  shows "part_solution cfg_side_T_ip_pkg x (side_sigma_at x) (side_stabl_at x)"
+  shows "part_solution cfg_side_T_ip_pkg x (side_nu_at x) (side_stabl_at x)"
   using side.partial_solution[OF dom side_solve_prod] by simp
 
 lemma side_query_in_stabl:
@@ -97,13 +97,13 @@ lemma side_entry_in_stabl:
 
 lemma side_solver_part_post_at_entry:
   assumes dom: "side.solve_dom (cfg_entry g)"
-  shows "part_post_solution cfg_side_T_ip_pkg (cfg_entry g) (side_sigma_at (cfg_entry g))
+  shows "part_post_solution cfg_side_T_ip_pkg (cfg_entry g) (side_nu_at (cfg_entry g))
            (side_stabl_at (cfg_entry g))"
   using side_part_post_solution_at[OF dom] by simp
 
 lemma side_solver_part_post_at:
   assumes dom: "side.solve_dom v0"
-  shows "part_post_solution cfg_side_T_ip_pkg v0 (side_sigma_at v0) (side_stabl_at v0)"
+  shows "part_post_solution cfg_side_T_ip_pkg v0 (side_nu_at v0) (side_stabl_at v0)"
   using side_part_post_solution_at[OF dom] by simp
 
 lemma side_solve_dom_eq:
@@ -112,11 +112,11 @@ lemma side_solve_dom_eq:
 
 lemma side_solver_part_post_at_cfg:
   assumes "side_cfg_ip_solve_dom g tf bot0 s0 v0"
-  shows "part_post_solution cfg_side_T_ip_pkg v0 (side_sigma_at v0) (side_stabl_at v0)"
+  shows "part_post_solution cfg_side_T_ip_pkg v0 (side_nu_at v0) (side_stabl_at v0)"
   using side_solver_part_post_at assms unfolding side_solve_dom_eq by simp
 
 lemma side_env_at_eq [simp]:
-  "side_env_at x0 v = side_env (side_sigma_at x0) v"
+  "side_env_at x0 v = side_env (side_nu_at x0) v"
   unfolding side_env_at_def by simp
 
 end
@@ -132,18 +132,18 @@ definition side_analyse_ip ::
      => pp
      => 'a abs_state"
 where
-  "side_analyse_ip pi ps main tf bot0 s0 v =
-     side_env (td_cfg_side_ip_solver.side_sigma_at (compile_prog pi ps main) tf bot0 s0 v) v"
+  "side_analyse_ip \<Pi> ps main tf bot0 s0 v =
+     side_env (td_cfg_side_ip_solver.side_nu_at (compile_prog \<Pi> ps main) tf bot0 s0 v) v"
 
 lemma side_analyse_ip_eq_env_at:
-  fixes pi ps main and tf :: "'a::bounded_semilattice_sup_bot domain_transfer"
+  fixes \<Pi> ps main and tf :: "'a::bounded_semilattice_sup_bot domain_transfer"
     and bot0 s0 :: "'a abs_state" and v :: pp
   assumes tf_mono:
     "\<And>a s1 s2. s1 \<le> s2 \<Longrightarrow> apply_tf tf a s1 \<le> apply_tf tf a s2"
-  shows "side_analyse_ip pi ps main tf bot0 s0 v =
-         td_cfg_side_ip_solver.side_env_at (compile_prog pi ps main) tf bot0 s0 v v"
+  shows "side_analyse_ip \<Pi> ps main tf bot0 s0 v =
+         td_cfg_side_ip_solver.side_env_at (compile_prog \<Pi> ps main) tf bot0 s0 v v"
 proof -
-  interpret side: td_cfg_side_ip_solver "compile_prog pi ps main" tf bot0 s0
+  interpret side: td_cfg_side_ip_solver "compile_prog \<Pi> ps main" tf bot0 s0
     using tf_mono by unfold_locales
   show ?thesis unfolding side_analyse_ip_def side.side_env_at_eq by simp
 qed
