src/Analysis/Domains/Interval_Side_IP_Soundness.thy
@@ -7,31 +7,31 @@ section \<open>Interval domain: side-effecting interprocedural TD solver instant
 text \<open>Instantiates the side IP solver (side_analyse_ip) at the Interval domain.\<close>
 
 theorem side_ip_ivl_analysis_sound:
-  fixes pi ps main and s t :: store and s0 :: "ivl abs_state"
+  fixes \<Pi> ps main and s t :: store and s0 :: "ivl abs_state"
   assumes s_sound: "s \<in> ivl_domain.gamma_state s0"
   assumes collect_exit:
-    "t \<in> cfg_collect_ip (compile_prog pi ps main) {s}
-       (cfg_exit (compile_prog pi ps main))"
+    "t \<in> cfg_collect_ip (compile_prog \<Pi> ps main) {s}
+       (cfg_exit (compile_prog \<Pi> ps main))"
   assumes side_solve_dom:
-    "side_cfg_ip_solve_dom (compile_prog pi ps main) ivl_tf bot s0
-       (cfg_exit (compile_prog pi ps main))"
+    "side_cfg_ip_solve_dom (compile_prog \<Pi> ps main) ivl_tf bot s0
+       (cfg_exit (compile_prog \<Pi> ps main))"
   shows "t \<in> ivl_domain.gamma_state
-       (side_analyse_ip pi ps main ivl_tf bot s0
-         (cfg_exit (compile_prog pi ps main)))"
+       (side_analyse_ip \<Pi> ps main ivl_tf bot s0
+         (cfg_exit (compile_prog \<Pi> ps main)))"
 proof -
   have gs: "{s} \<le> sound_domain.gamma_state gamma_ivl s0"
     using s_sound
     unfolding ivl_domain.gamma_state_def sound_domain.gamma_state_def by auto
   have collect:
-    "cfg_collect_ip (compile_prog pi ps main) {s} (cfg_exit (compile_prog pi ps main))
+    "cfg_collect_ip (compile_prog \<Pi> ps main) {s} (cfg_exit (compile_prog \<Pi> ps main))
      \<le> sound_domain.gamma_state gamma_ivl
-         (side_analyse_ip pi ps main ivl_tf bot s0
-           (cfg_exit (compile_prog pi ps main)))"
+         (side_analyse_ip \<Pi> ps main ivl_tf bot s0
+           (cfg_exit (compile_prog \<Pi> ps main)))"
     by (rule sound_transfer.side_analyse_ip_collect_sound_exit_pruned
           [OF ivl_sound_tf.sound_transfer_axioms ivl_tf_mono side_solve_dom gs])
   have "t \<in> sound_domain.gamma_state gamma_ivl
-       (side_analyse_ip pi ps main ivl_tf bot s0
-         (cfg_exit (compile_prog pi ps main)))"
+       (side_analyse_ip \<Pi> ps main ivl_tf bot s0
+         (cfg_exit (compile_prog \<Pi> ps main)))"
     using collect collect_exit by blast
   then show ?thesis
     unfolding ivl_domain.gamma_state_def sound_domain.gamma_state_def by auto
