src/Analysis/Equations/Constraint_System_IP_Sound.thy
@@ -61,9 +61,9 @@ lemma combine_states_sound:
   assumes sc: "s \<in> gamma_state \<sigma>c" and se: "t \<in> gamma_state \<sigma>e"
   shows "combine_states s t \<in> gamma_state (combine_abs \<sigma>c \<sigma>e)"
 proof -
-  from sc have Vc: "\<forall>z. s z \<in> gamma (\<sigma>c z)"
+  from sc have Vc: "\<forall>z. s z \<in> \<gamma> (\<sigma>c z)"
     unfolding gamma_state_def by auto
-  from se have Ve: "\<forall>z. t z \<in> gamma (\<sigma>e z)"
+  from se have Ve: "\<forall>z. t z \<in> \<gamma> (\<sigma>e z)"
     unfolding gamma_state_def by auto
   show ?thesis unfolding gamma_state_def combine_abs_def combine_states_def
     using Vc Ve by auto
