src/Analysis/Solver/TD_Side_IP_Bounds.thy
@@ -21,27 +21,27 @@ subsection \<open>Post-solution in usable form\<close>
    the local fold by the local unknown and the global contribution by the
    single global unknown. *)
 lemma side_post_solution_le_local_ip:
-  assumes "part_post_solution (side_cfg_T_ip g tf (\<squnion>) bot0 s0) x sigma vars"
+  assumes "part_post_solution (side_cfg_T_ip g tf (\<squnion>) bot0 s0) x \<sigma> vars"
       and "v \<in> vars"
   shows "side_acc_ip tf (\<squnion>)
            (if v = cfg_entry g then bot0 \<squnion> restrict_local s0 else bot0)
-           sigma (predecessor_list g v) (combine_predecessor_list g v) \<le> sigma (Inl v)"
+           \<sigma> (predecessor_list g v) (combine_predecessor_list g v) \<le> \<sigma> (Inl v)"
 proof -
-  from assms have "eq (side_cfg_T_ip g tf (\<squnion>) bot0 s0) v sigma \<le> sigma (Inl v)" by auto
+  from assms have "eq (side_cfg_T_ip g tf (\<squnion>) bot0 s0) v \<sigma> \<le> \<sigma> (Inl v)" by auto
   thus ?thesis by (simp add: eq_side_cfg_T_ip)
 qed
 
 lemma side_post_solution_le_global_ip:
-  assumes "part_post_solution (side_cfg_T_ip g tf (\<squnion>) bot0 s0) x sigma vars"
+  assumes "part_post_solution (side_cfg_T_ip g tf (\<squnion>) bot0 s0) x \<sigma> vars"
       and "v \<in> vars"
-  shows "side_glob_ip tf (\<squnion>) sigma (predecessor_list g v) (combine_predecessor_list g v)
-         \<le> sigma (Inr ())"
+  shows "side_glob_ip tf (\<squnion>) \<sigma> (predecessor_list g v) (combine_predecessor_list g v)
+         \<le> \<sigma> (Inr ())"
 proof -
-  from assms have "sides_of_rhs (side_cfg_T_ip g tf (\<squnion>) bot0 s0 v) sigma \<le> sigma" by auto
-  hence le: "sides_of_rhs (side_cfg_T_ip g tf (\<squnion>) bot0 s0 v) sigma (Inr ()) \<le> sigma (Inr ())"
+  from assms have "sides_of_rhs (side_cfg_T_ip g tf (\<squnion>) bot0 s0 v) \<sigma> \<le> \<sigma>" by auto
+  hence le: "sides_of_rhs (side_cfg_T_ip g tf (\<squnion>) bot0 s0 v) \<sigma> (Inr ()) \<le> \<sigma> (Inr ())"
     by (simp add: le_fun_def)
-  have "side_glob_ip tf (\<squnion>) sigma (predecessor_list g v) (combine_predecessor_list g v)
-        \<le> sides_of_rhs (side_cfg_T_ip g tf (\<squnion>) bot0 s0 v) sigma (Inr ())"
+  have "side_glob_ip tf (\<squnion>) \<sigma> (predecessor_list g v) (combine_predecessor_list g v)
+        \<le> sides_of_rhs (side_cfg_T_ip g tf (\<squnion>) bot0 s0 v) \<sigma> (Inr ())"
     unfolding side_cfg_T_ip_def
     by (simp add: sides_make_side_rhs_tree_ip_Inr)
   thus ?thesis using le by (rule order_trans)
@@ -50,7 +50,7 @@ qed
 subsection \<open>Fold upper bounds (join = sup)\<close>
 
 lemma side_acc_ip_ge_acc:
-  "acc \<le> side_acc_ip tf (\<squnion>) acc sigma es cs"
+  "acc \<le> side_acc_ip tf (\<squnion>) acc \<sigma> es cs"
 proof (induction es arbitrary: acc cs)
   case Nil
   show ?case
@@ -60,7 +60,7 @@ proof (induction es arbitrary: acc cs)
     case (Cons x cs)
     obtain cc ex where x: "x = (cc, ex)" by (cases x)
     have "acc \<le> side_acc_ip tf (\<squnion>)
-            (acc \<squnion> restrict_local (sigma (Inl cc) \<squnion> sigma (Inr ()))) sigma [] cs"
+            (acc \<squnion> restrict_local (\<sigma> (Inl cc) \<squnion> \<sigma> (Inr ()))) \<sigma> [] cs"
       by (meson Cons.IH sup_ge1 order_trans)
     then show ?case unfolding x by (simp only: side_acc_ip.simps)
   qed
@@ -68,25 +68,25 @@ next
   case (Cons x es)
   obtain u a where x: "x = (u, a)" by (cases x)
   have "acc \<le> side_acc_ip tf (\<squnion>)
-          (acc \<squnion> restrict_local (apply_tf tf a (sigma (Inl u) \<squnion> sigma (Inr ())))) sigma es cs"
+          (acc \<squnion> restrict_local (apply_tf tf a (\<sigma> (Inl u) \<squnion> \<sigma> (Inr ())))) \<sigma> es cs"
     by (meson Cons.IH sup_ge1 order_trans)
   then show ?case unfolding x by (simp only: side_acc_ip.simps)
 qed
 
 (* The local fold grows monotonically as more incoming edges are processed. *)
 lemma side_acc_ip_es_mono:
-  "side_acc_ip tf (\<squnion>) acc sigma [] cs \<le> side_acc_ip tf (\<squnion>) acc sigma es cs"
+  "side_acc_ip tf (\<squnion>) acc \<sigma> [] cs \<le> side_acc_ip tf (\<squnion>) acc \<sigma> es cs"
 proof (induction es arbitrary: acc)
   case Nil show ?case by simp
 next
   case (Cons x es)
   obtain u a where x: "x = (u, a)" by (cases x)
-  have "side_acc_ip tf (\<squnion>) acc sigma [] cs
+  have "side_acc_ip tf (\<squnion>) acc \<sigma> [] cs
         \<le> side_acc_ip tf (\<squnion>)
-            (acc \<squnion> restrict_local (apply_tf tf a (sigma (Inl u) \<squnion> sigma (Inr ())))) sigma [] cs"
+            (acc \<squnion> restrict_local (apply_tf tf a (\<sigma> (Inl u) \<squnion> \<sigma> (Inr ())))) \<sigma> [] cs"
     by (rule side_acc_ip_mono_acc[OF sup_mono sup_ge1])
   also have "... \<le> side_acc_ip tf (\<squnion>)
-            (acc \<squnion> restrict_local (apply_tf tf a (sigma (Inl u) \<squnion> sigma (Inr ())))) sigma es cs"
+            (acc \<squnion> restrict_local (apply_tf tf a (\<sigma> (Inl u) \<squnion> \<sigma> (Inr ())))) \<sigma> es cs"
     by (rule Cons.IH)
   finally show ?case unfolding x by (simp only: side_acc_ip.simps)
 qed
@@ -94,8 +94,8 @@ qed
 (* Each incoming edge's local contribution is below the local fold. *)
 lemma restrict_local_le_side_acc_ip_edge:
   "(u, a) \<in> set es \<Longrightarrow>
-   restrict_local (apply_tf tf a (sigma (Inl u) \<squnion> sigma (Inr ())))
-     \<le> side_acc_ip tf (\<squnion>) acc sigma es cs"
+   restrict_local (apply_tf tf a (\<sigma> (Inl u) \<squnion> \<sigma> (Inr ())))
+     \<le> side_acc_ip tf (\<squnion>) acc \<sigma> es cs"
 proof (induction es arbitrary: acc)
   case Nil thus ?case by simp
 next
@@ -106,18 +106,18 @@ next
   proof cases
     case hd
     then have uw: "u = w" and ab: "a = b" by auto
-    have "restrict_local (apply_tf tf b (sigma (Inl w) \<squnion> sigma (Inr ())))
+    have "restrict_local (apply_tf tf b (\<sigma> (Inl w) \<squnion> \<sigma> (Inr ())))
           \<le> side_acc_ip tf (\<squnion>)
-               (acc \<squnion> restrict_local (apply_tf tf b (sigma (Inl w) \<squnion> sigma (Inr ()))))
-               sigma es cs"
+               (acc \<squnion> restrict_local (apply_tf tf b (\<sigma> (Inl w) \<squnion> \<sigma> (Inr ()))))
+               \<sigma> es cs"
       using side_acc_ip_ge_acc sup_ge2 order_trans by blast
     thus ?thesis unfolding x uw ab by (simp only: side_acc_ip.simps)
   next
     case tl
-    have "restrict_local (apply_tf tf a (sigma (Inl u) \<squnion> sigma (Inr ())))
+    have "restrict_local (apply_tf tf a (\<sigma> (Inl u) \<squnion> \<sigma> (Inr ())))
           \<le> side_acc_ip tf (\<squnion>)
-               (acc \<squnion> restrict_local (apply_tf tf b (sigma (Inl w) \<squnion> sigma (Inr ()))))
-               sigma es cs"
+               (acc \<squnion> restrict_local (apply_tf tf b (\<sigma> (Inl w) \<squnion> \<sigma> (Inr ()))))
+               \<sigma> es cs"
       by (rule Cons.IH[OF tl])
     thus ?thesis unfolding x by (simp only: side_acc_ip.simps)
   qed
@@ -127,8 +127,8 @@ qed
    local fold (edge list exhausted). *)
 lemma restrict_local_le_side_acc_ip_combine_nil:
   "(cc, ex) \<in> set cs \<Longrightarrow>
-   restrict_local (sigma (Inl cc) \<squnion> sigma (Inr ()))
-     \<le> side_acc_ip tf (\<squnion>) acc sigma [] cs"
+   restrict_local (\<sigma> (Inl cc) \<squnion> \<sigma> (Inr ()))
+     \<le> side_acc_ip tf (\<squnion>) acc \<sigma> [] cs"
 proof (induction cs arbitrary: acc)
   case Nil thus ?case by simp
 next
@@ -139,16 +139,16 @@ next
   proof cases
     case hd
     then have cc2: "cc = c2" and exe2: "ex = e2" by auto
-    have "restrict_local (sigma (Inl c2) \<squnion> sigma (Inr ()))
+    have "restrict_local (\<sigma> (Inl c2) \<squnion> \<sigma> (Inr ()))
           \<le> side_acc_ip tf (\<squnion>)
-               (acc \<squnion> restrict_local (sigma (Inl c2) \<squnion> sigma (Inr ()))) sigma [] cs"
+               (acc \<squnion> restrict_local (\<sigma> (Inl c2) \<squnion> \<sigma> (Inr ()))) \<sigma> [] cs"
       using side_acc_ip_ge_acc sup_ge2 order_trans by blast
     thus ?thesis unfolding x cc2 exe2 by (simp only: side_acc_ip.simps)
   next
     case tl
-    have "restrict_local (sigma (Inl cc) \<squnion> sigma (Inr ()))
+    have "restrict_local (\<sigma> (Inl cc) \<squnion> \<sigma> (Inr ()))
           \<le> side_acc_ip tf (\<squnion>)
-               (acc \<squnion> restrict_local (sigma (Inl c2) \<squnion> sigma (Inr ()))) sigma [] cs"
+               (acc \<squnion> restrict_local (\<sigma> (Inl c2) \<squnion> \<sigma> (Inr ()))) \<sigma> [] cs"
       by (rule Cons.IH[OF tl])
     thus ?thesis unfolding x by (simp only: side_acc_ip.simps)
   qed
@@ -156,31 +156,31 @@ qed
 
 lemma restrict_local_le_side_acc_ip_combine:
   assumes "(cc, ex) \<in> set cs"
-  shows "restrict_local (sigma (Inl cc) \<squnion> sigma (Inr ()))
-         \<le> side_acc_ip tf (\<squnion>) acc sigma es cs"
+  shows "restrict_local (\<sigma> (Inl cc) \<squnion> \<sigma> (Inr ()))
+         \<le> side_acc_ip tf (\<squnion>) acc \<sigma> es cs"
   using restrict_local_le_side_acc_ip_combine_nil[OF assms] side_acc_ip_es_mono
   by (rule order_trans)
 
 (* Global fold analogues. *)
 lemma side_glob_ip_es_mono:
-  "side_glob_ip tf (\<squnion>) sigma [] cs \<le> side_glob_ip tf (\<squnion>) sigma es cs"
+  "side_glob_ip tf (\<squnion>) \<sigma> [] cs \<le> side_glob_ip tf (\<squnion>) \<sigma> es cs"
 proof (induction es)
   case Nil show ?case by simp
 next
   case (Cons x es)
   obtain u a where x: "x = (u, a)" by (cases x)
-  have "side_glob_ip tf (\<squnion>) sigma [] cs \<le> side_glob_ip tf (\<squnion>) sigma es cs"
+  have "side_glob_ip tf (\<squnion>) \<sigma> [] cs \<le> side_glob_ip tf (\<squnion>) \<sigma> es cs"
     by (rule Cons.IH)
-  also have "... \<le> side_glob_ip tf (\<squnion>) sigma es cs
-                     \<squnion> restrict_global (apply_tf tf a (sigma (Inl u) \<squnion> sigma (Inr ())))"
+  also have "... \<le> side_glob_ip tf (\<squnion>) \<sigma> es cs
+                     \<squnion> restrict_global (apply_tf tf a (\<sigma> (Inl u) \<squnion> \<sigma> (Inr ())))"
     by (rule sup_ge1)
   finally show ?case unfolding x by (simp only: side_glob_ip.simps)
 qed
 
 lemma restrict_global_le_side_glob_ip_edge:
   "(u, a) \<in> set es \<Longrightarrow>
-   restrict_global (apply_tf tf a (sigma (Inl u) \<squnion> sigma (Inr ())))
-     \<le> side_glob_ip tf (\<squnion>) sigma es cs"
+   restrict_global (apply_tf tf a (\<sigma> (Inl u) \<squnion> \<sigma> (Inr ())))
+     \<le> side_glob_ip tf (\<squnion>) \<sigma> es cs"
 proof (induction es)
   case Nil thus ?case by simp
 next
@@ -191,16 +191,16 @@ next
   proof cases
     case hd
     then have uw: "u = w" and ab: "a = b" by auto
-    have "restrict_global (apply_tf tf b (sigma (Inl w) \<squnion> sigma (Inr ())))
-          \<le> side_glob_ip tf (\<squnion>) sigma es cs
-               \<squnion> restrict_global (apply_tf tf b (sigma (Inl w) \<squnion> sigma (Inr ())))"
+    have "restrict_global (apply_tf tf b (\<sigma> (Inl w) \<squnion> \<sigma> (Inr ())))
+          \<le> side_glob_ip tf (\<squnion>) \<sigma> es cs
+               \<squnion> restrict_global (apply_tf tf b (\<sigma> (Inl w) \<squnion> \<sigma> (Inr ())))"
       by (rule sup_ge2)
     thus ?thesis unfolding x uw ab by (simp only: side_glob_ip.simps)
   next
     case tl
-    have "restrict_global (apply_tf tf a (sigma (Inl u) \<squnion> sigma (Inr ())))
-          \<le> side_glob_ip tf (\<squnion>) sigma es cs
-               \<squnion> restrict_global (apply_tf tf b (sigma (Inl w) \<squnion> sigma (Inr ())))"
+    have "restrict_global (apply_tf tf a (\<sigma> (Inl u) \<squnion> \<sigma> (Inr ())))
+          \<le> side_glob_ip tf (\<squnion>) \<sigma> es cs
+               \<squnion> restrict_global (apply_tf tf b (\<sigma> (Inl w) \<squnion> \<sigma> (Inr ())))"
       using Cons.IH[OF tl] by (rule le_supI1)
     thus ?thesis unfolding x by (simp only: side_glob_ip.simps)
   qed
@@ -208,8 +208,8 @@ qed
 
 lemma restrict_global_le_side_glob_ip_combine_nil:
   "(cc, ex) \<in> set cs \<Longrightarrow>
-   restrict_global (sigma (Inl ex) \<squnion> sigma (Inr ()))
-     \<le> side_glob_ip tf (\<squnion>) sigma [] cs"
+   restrict_global (\<sigma> (Inl ex) \<squnion> \<sigma> (Inr ()))
+     \<le> side_glob_ip tf (\<squnion>) \<sigma> [] cs"
 proof (induction cs)
   case Nil thus ?case by simp
 next
@@ -220,16 +220,16 @@ next
   proof cases
     case hd
     then have exe2: "ex = e2" by auto
-    have "restrict_global (sigma (Inl e2) \<squnion> sigma (Inr ()))
-          \<le> side_glob_ip tf (\<squnion>) sigma [] cs
-               \<squnion> restrict_global (sigma (Inl e2) \<squnion> sigma (Inr ()))"
+    have "restrict_global (\<sigma> (Inl e2) \<squnion> \<sigma> (Inr ()))
+          \<le> side_glob_ip tf (\<squnion>) \<sigma> [] cs
+               \<squnion> restrict_global (\<sigma> (Inl e2) \<squnion> \<sigma> (Inr ()))"
       by (rule sup_ge2)
     thus ?thesis unfolding x exe2 by (simp only: side_glob_ip.simps)
   next
     case tl
-    have "restrict_global (sigma (Inl ex) \<squnion> sigma (Inr ()))
-          \<le> side_glob_ip tf (\<squnion>) sigma [] cs
-               \<squnion> restrict_global (sigma (Inl e2) \<squnion> sigma (Inr ()))"
+    have "restrict_global (\<sigma> (Inl ex) \<squnion> \<sigma> (Inr ()))
+          \<le> side_glob_ip tf (\<squnion>) \<sigma> [] cs
+               \<squnion> restrict_global (\<sigma> (Inl e2) \<squnion> \<sigma> (Inr ()))"
       using Cons.IH[OF tl] by (rule le_supI1)
     thus ?thesis unfolding x by (simp only: side_glob_ip.simps)
   qed
@@ -237,8 +237,8 @@ qed
 
 lemma restrict_global_le_side_glob_ip_combine:
   assumes "(cc, ex) \<in> set cs"
-  shows "restrict_global (sigma (Inl ex) \<squnion> sigma (Inr ()))
-         \<le> side_glob_ip tf (\<squnion>) sigma es cs"
+  shows "restrict_global (\<sigma> (Inl ex) \<squnion> \<sigma> (Inr ()))
+         \<le> side_glob_ip tf (\<squnion>) \<sigma> es cs"
   using restrict_global_le_side_glob_ip_combine_nil[OF assms] side_glob_ip_es_mono
   by (rule order_trans)
 
@@ -247,25 +247,25 @@ subsection \<open>Edge / combine closure of a side post-solution\<close>
 (* For any CFG edge (u, a, v), a post-solution's combined env at u, transferred
    along a, is below the combined env at v. *)
 lemma apply_tf_combined_le_ip:
-  assumes pp:  "part_post_solution (side_cfg_T_ip g tf (\<squnion>) bot0 s0) x sigma vars"
+  assumes pp:  "part_post_solution (side_cfg_T_ip g tf (\<squnion>) bot0 s0) x \<sigma> vars"
       and v:   "v \<in> vars"
       and e:   "(u, a, v) \<in> edges g"
       and fin: "finite (edges g)"
-  shows "apply_tf tf a (side_env sigma u) \<le> side_env sigma v"
+  shows "apply_tf tf a (side_env \<sigma> u) \<le> side_env \<sigma> v"
 proof -
   have mem: "(u, a) \<in> set (predecessor_list g v)"
     using e by (simp add: set_predecessor_list[OF fin] predecessors_def)
-  have loc: "restrict_local (apply_tf tf a (side_env sigma u)) \<le> sigma (Inl v)"
+  have loc: "restrict_local (apply_tf tf a (side_env \<sigma> u)) \<le> \<sigma> (Inl v)"
     using restrict_local_le_side_acc_ip_edge[OF mem] side_post_solution_le_local_ip[OF pp v]
     unfolding side_env_def by (rule order_trans)
-  have glob: "restrict_global (apply_tf tf a (side_env sigma u)) \<le> sigma (Inr ())"
+  have glob: "restrict_global (apply_tf tf a (side_env \<sigma> u)) \<le> \<sigma> (Inr ())"
     using restrict_global_le_side_glob_ip_edge[OF mem] side_post_solution_le_global_ip[OF pp v]
     unfolding side_env_def by (rule order_trans)
-  have "apply_tf tf a (side_env sigma u)
-        = restrict_local (apply_tf tf a (side_env sigma u))
-          \<squnion> restrict_global (apply_tf tf a (side_env sigma u))"
+  have "apply_tf tf a (side_env \<sigma> u)
+        = restrict_local (apply_tf tf a (side_env \<sigma> u))
+          \<squnion> restrict_global (apply_tf tf a (side_env \<sigma> u))"
     by (rule restrict_local_global_join[symmetric])
-  also have "... \<le> sigma (Inl v) \<squnion> sigma (Inr ())"
+  also have "... \<le> \<sigma> (Inl v) \<squnion> \<sigma> (Inr ())"
     using loc glob by (rule sup_mono)
   finally show ?thesis unfolding side_env_def .
 qed
@@ -275,26 +275,26 @@ qed
    at the return point v. *)
 lemma combine_combined_le_ip:
   fixes g :: cfg and tf :: "'a::bounded_semilattice_sup_bot domain_transfer"
-    and bot0 s0 :: "'a abs_state" and sigma :: "pp + unit \<Rightarrow> 'a abs_state"
+    and bot0 s0 :: "'a abs_state" and \<sigma> :: "pp + unit \<Rightarrow> 'a abs_state"
     and c ex v :: pp
-  assumes pp:   "part_post_solution (side_cfg_T_ip g tf (\<squnion>) bot0 s0) x sigma vars"
+  assumes pp:   "part_post_solution (side_cfg_T_ip g tf (\<squnion>) bot0 s0) x \<sigma> vars"
       and v:    "v \<in> vars"
       and e:    "(c, ex, v) \<in> combines g"
       and finC: "finite (combines g)"
-  shows "combine_abs (side_env sigma c) (side_env sigma ex) \<le> side_env sigma v"
+  shows "combine_abs (side_env \<sigma> c) (side_env \<sigma> ex) \<le> side_env \<sigma> v"
 proof -
   have mem: "(c, ex) \<in> set (combine_predecessor_list g v)"
     using e by (simp add: set_combine_predecessor_list[OF finC] combine_predecessors_def)
-  have loc: "restrict_local (side_env sigma c) \<le> sigma (Inl v)"
+  have loc: "restrict_local (side_env \<sigma> c) \<le> \<sigma> (Inl v)"
     using restrict_local_le_side_acc_ip_combine[OF mem] side_post_solution_le_local_ip[OF pp v]
     unfolding side_env_def by (rule order_trans)
-  have glob: "restrict_global (side_env sigma ex) \<le> sigma (Inr ())"
+  have glob: "restrict_global (side_env \<sigma> ex) \<le> \<sigma> (Inr ())"
     using restrict_global_le_side_glob_ip_combine[OF mem] side_post_solution_le_global_ip[OF pp v]
     unfolding side_env_def by (rule order_trans)
-  have "combine_abs (side_env sigma c) (side_env sigma ex)
-        = restrict_local (side_env sigma c) \<squnion> restrict_global (side_env sigma ex)"
+  have "combine_abs (side_env \<sigma> c) (side_env \<sigma> ex)
+        = restrict_local (side_env \<sigma> c) \<squnion> restrict_global (side_env \<sigma> ex)"
     by (simp add: combine_abs_def restrict_combine)
-  also have "... \<le> sigma (Inl v) \<squnion> sigma (Inr ())"
+  also have "... \<le> \<sigma> (Inl v) \<squnion> \<sigma> (Inr ())"
     using loc glob by (rule sup_mono)
   finally show ?thesis unfolding side_env_def .
 qed
@@ -303,7 +303,7 @@ subsection \<open>Dependency membership (edges and combine endpoints)\<close>
 
 lemma Inl_dep_aux_side_rhs_fold_ip_edge:
   assumes "(u, a) \<in> set es"
-  shows "Inl u \<in> dep_aux sigma (side_rhs_fold_ip tf join acc es cs)"
+  shows "Inl u \<in> dep_aux \<sigma> (side_rhs_fold_ip tf join acc es cs)"
   using assms
 proof (induction es arbitrary: acc)
   case Nil thus ?case by simp
@@ -325,20 +325,20 @@ qed
 (* The dependencies reachable after the edge list is exhausted (the combine
    queries) survive the edge prefix. *)
 lemma dep_aux_side_rhs_fold_ip_nil_sub_es:
-  "dep_aux sigma (side_rhs_fold_ip tf join acc [] cs)
-   \<subseteq> dep_aux sigma (side_rhs_fold_ip tf join acc es cs)"
+  "dep_aux \<sigma> (side_rhs_fold_ip tf join acc [] cs)
+   \<subseteq> dep_aux \<sigma> (side_rhs_fold_ip tf join acc es cs)"
 proof (induction es arbitrary: acc)
   case Nil show ?case by simp
 next
   case (Cons x es)
   obtain w b where x: "x = (w, b)" by (cases x)
-  let ?acc' = "join acc (restrict_local (apply_tf tf b (join (sigma (Inl w)) (sigma (Inr ())))))"
-  have "dep_aux sigma (side_rhs_fold_ip tf join acc [] cs)
-        = dep_aux sigma (side_rhs_fold_ip tf join ?acc' [] cs)"
+  let ?acc' = "join acc (restrict_local (apply_tf tf b (join (\<sigma> (Inl w)) (\<sigma> (Inr ())))))"
+  have "dep_aux \<sigma> (side_rhs_fold_ip tf join acc [] cs)
+        = dep_aux \<sigma> (side_rhs_fold_ip tf join ?acc' [] cs)"
     by (rule dep_aux_side_rhs_fold_ip_acc_indep)
-  also have "... \<subseteq> dep_aux sigma (side_rhs_fold_ip tf join ?acc' es cs)"
+  also have "... \<subseteq> dep_aux \<sigma> (side_rhs_fold_ip tf join ?acc' es cs)"
     by (rule Cons.IH)
-  also have "... \<subseteq> dep_aux sigma (side_rhs_fold_ip tf join acc (x # es) cs)"
+  also have "... \<subseteq> dep_aux \<sigma> (side_rhs_fold_ip tf join acc (x # es) cs)"
     unfolding x side_rhs_fold_ip.simps dep_aux.simps Let_def by auto
   finally show ?case .
 qed
@@ -346,9 +346,9 @@ qed
 lemma Inl_dep_aux_side_rhs_fold_ip_call:
   fixes c ex :: pp
   assumes "(c, ex) \<in> set cs"
-  shows "Inl c \<in> dep_aux sigma (side_rhs_fold_ip tf join acc es cs)"
+  shows "Inl c \<in> dep_aux \<sigma> (side_rhs_fold_ip tf join acc es cs)"
 proof -
-  have "Inl c \<in> dep_aux sigma (side_rhs_fold_ip tf join acc [] cs)"
+  have "Inl c \<in> dep_aux \<sigma> (side_rhs_fold_ip tf join acc [] cs)"
     using assms
   proof (induction cs arbitrary: acc)
     case Nil thus ?case by simp
@@ -372,9 +372,9 @@ qed
 lemma Inl_dep_aux_side_rhs_fold_ip_exit:
   fixes c ex :: pp
   assumes "(c, ex) \<in> set cs"
-  shows "Inl ex \<in> dep_aux sigma (side_rhs_fold_ip tf join acc es cs)"
+  shows "Inl ex \<in> dep_aux \<sigma> (side_rhs_fold_ip tf join acc es cs)"
 proof -
-  have "Inl ex \<in> dep_aux sigma (side_rhs_fold_ip tf join acc [] cs)"
+  have "Inl ex \<in> dep_aux \<sigma> (side_rhs_fold_ip tf join acc [] cs)"
     using assms
   proof (induction cs arbitrary: acc)
     case Nil thus ?case by simp
@@ -400,11 +400,11 @@ subsection \<open>Dependency at the eqsT level (edges and combine endpoints)\<cl
 lemma dep_side_rhs_tree_ip_edge:
   assumes fin: "finite (edges g)"
   assumes ed: "(u, a, w) \<in> edges g"
-  shows "u \<in> dep\<^sub>L (side_cfg_T_ip g tf join bot0 s0) sigma w"
+  shows "u \<in> dep\<^sub>L (side_cfg_T_ip g tf join bot0 s0) \<sigma> w"
 proof -
   have mem: "(u, a) \<in> set (predecessor_list g w)"
     using ed fin by (auto simp: predecessors_def set_predecessor_list)
-  have "Inl u \<in> dep_aux sigma (make_side_rhs_tree_ip g tf join bot0 s0 w)"
+  have "Inl u \<in> dep_aux \<sigma> (make_side_rhs_tree_ip g tf join bot0 s0 w)"
     unfolding dep_aux_make_side_rhs_tree_ip
     by (rule Inl_dep_aux_side_rhs_fold_ip_edge[OF mem])
   thus ?thesis unfolding side_cfg_T_ip_def dep\<^sub>L_def dep_def by simp
@@ -414,15 +414,15 @@ lemma dep_side_rhs_tree_ip_combine:
   fixes g :: cfg and c ex w :: pp
   assumes finC: "finite (combines g)"
   assumes ce: "(c, ex, w) \<in> combines g"
-  shows "c \<in> dep\<^sub>L (side_cfg_T_ip g tf join bot0 s0) sigma w
-       \<and> ex \<in> dep\<^sub>L (side_cfg_T_ip g tf join bot0 s0) sigma w"
+  shows "c \<in> dep\<^sub>L (side_cfg_T_ip g tf join bot0 s0) \<sigma> w
+       \<and> ex \<in> dep\<^sub>L (side_cfg_T_ip g tf join bot0 s0) \<sigma> w"
 proof -
   have mem: "(c, ex) \<in> set (combine_predecessor_list g w)"
     using ce finC by (simp add: combine_predecessors_def)
-  have dc: "Inl c \<in> dep_aux sigma (make_side_rhs_tree_ip g tf join bot0 s0 w)"
+  have dc: "Inl c \<in> dep_aux \<sigma> (make_side_rhs_tree_ip g tf join bot0 s0 w)"
     unfolding dep_aux_make_side_rhs_tree_ip
     by (rule Inl_dep_aux_side_rhs_fold_ip_call[OF mem])
-  have de: "Inl ex \<in> dep_aux sigma (make_side_rhs_tree_ip g tf join bot0 s0 w)"
+  have de: "Inl ex \<in> dep_aux \<sigma> (make_side_rhs_tree_ip g tf join bot0 s0 w)"
     unfolding dep_aux_make_side_rhs_tree_ip
     by (rule Inl_dep_aux_side_rhs_fold_ip_exit[OF mem])
   show ?thesis using dc de unfolding side_cfg_T_ip_def dep\<^sub>L_def dep_def by simp
@@ -434,23 +434,23 @@ subsection \<open>Entry coverage from an arbitrary initial state\<close>
    single global unknown, so the initial globals are below it in any
    post-solution. *)
 lemma restrict_global_s0_le_global_ip:
-  assumes pp: "part_post_solution (side_cfg_T_ip g tf (\<squnion>) bot0 s0) x sigma vars"
+  assumes pp: "part_post_solution (side_cfg_T_ip g tf (\<squnion>) bot0 s0) x \<sigma> vars"
       and entry_in: "cfg_entry g \<in> vars"
-  shows "restrict_global s0 \<le> sigma (Inr ())"
+  shows "restrict_global s0 \<le> \<sigma> (Inr ())"
 proof -
-  from pp entry_in have "sides_of_rhs (side_cfg_T_ip g tf (\<squnion>) bot0 s0 (cfg_entry g)) sigma \<le> sigma"
+  from pp entry_in have "sides_of_rhs (side_cfg_T_ip g tf (\<squnion>) bot0 s0 (cfg_entry g)) \<sigma> \<le> \<sigma>"
     by auto
-  hence le: "sides_of_rhs (side_cfg_T_ip g tf (\<squnion>) bot0 s0 (cfg_entry g)) sigma (Inr ())
-             \<le> sigma (Inr ())"
+  hence le: "sides_of_rhs (side_cfg_T_ip g tf (\<squnion>) bot0 s0 (cfg_entry g)) \<sigma> (Inr ())
+             \<le> \<sigma> (Inr ())"
     by (simp add: le_fun_def)
   have "restrict_global s0
-        \<le> side_glob_ip tf (\<squnion>) sigma
+        \<le> side_glob_ip tf (\<squnion>) \<sigma>
              (predecessor_list g (cfg_entry g)) (combine_predecessor_list g (cfg_entry g))
            \<squnion> restrict_global s0"
     by (rule sup_ge2)
-  also have "... = sides_of_rhs (side_cfg_T_ip g tf (\<squnion>) bot0 s0 (cfg_entry g)) sigma (Inr ())"
+  also have "... = sides_of_rhs (side_cfg_T_ip g tf (\<squnion>) bot0 s0 (cfg_entry g)) \<sigma> (Inr ())"
     unfolding side_cfg_T_ip_def by (simp add: sides_make_side_rhs_tree_ip_Inr)
-  also have "... \<le> sigma (Inr ())" by (rule le)
+  also have "... \<le> \<sigma> (Inr ())" by (rule le)
   finally show ?thesis .
 qed
 
@@ -458,25 +458,25 @@ qed
    Side () seeds restrict_global s0, so s0 itself is below the combined env at
    the entry -- for an arbitrary initial state, no globals-free hypothesis. *)
 lemma s0_le_side_env_entry_ip:
-  assumes pp: "part_post_solution (side_cfg_T_ip g tf (\<squnion>) bot s0) v0 sigma vars"
+  assumes pp: "part_post_solution (side_cfg_T_ip g tf (\<squnion>) bot s0) v0 \<sigma> vars"
   assumes entry_in: "cfg_entry g \<in> vars"
-  shows "s0 \<le> side_env sigma (cfg_entry g)"
+  shows "s0 \<le> side_env \<sigma> (cfg_entry g)"
 proof -
-  have acc_le: "side_acc_ip tf (\<squnion>) (bot \<squnion> restrict_local s0) sigma
+  have acc_le: "side_acc_ip tf (\<squnion>) (bot \<squnion> restrict_local s0) \<sigma>
                   (predecessor_list g (cfg_entry g)) (combine_predecessor_list g (cfg_entry g))
-                \<le> sigma (Inl (cfg_entry g))"
+                \<le> \<sigma> (Inl (cfg_entry g))"
     using side_post_solution_le_local_ip[OF pp entry_in] by simp
   have "restrict_local s0 \<le> bot \<squnion> restrict_local s0" by simp
-  also have "... \<le> side_acc_ip tf (\<squnion>) (bot \<squnion> restrict_local s0) sigma
+  also have "... \<le> side_acc_ip tf (\<squnion>) (bot \<squnion> restrict_local s0) \<sigma>
                      (predecessor_list g (cfg_entry g)) (combine_predecessor_list g (cfg_entry g))"
     by (rule side_acc_ip_ge_acc)
-  also have "... \<le> sigma (Inl (cfg_entry g))" by (rule acc_le)
-  finally have rl: "restrict_local s0 \<le> sigma (Inl (cfg_entry g))" .
-  have rg: "restrict_global s0 \<le> sigma (Inr ())"
+  also have "... \<le> \<sigma> (Inl (cfg_entry g))" by (rule acc_le)
+  finally have rl: "restrict_local s0 \<le> \<sigma> (Inl (cfg_entry g))" .
+  have rg: "restrict_global s0 \<le> \<sigma> (Inr ())"
     by (rule restrict_global_s0_le_global_ip[OF pp entry_in])
   have "s0 = restrict_local s0 \<squnion> restrict_global s0"
     by (rule restrict_local_global_join[symmetric])
-  also have "... \<le> sigma (Inl (cfg_entry g)) \<squnion> sigma (Inr ())"
+  also have "... \<le> \<sigma> (Inl (cfg_entry g)) \<squnion> \<sigma> (Inr ())"
     using rl rg by (rule sup_mono)
   finally show ?thesis unfolding side_env_def .
 qed
